KripkeGameAnalysis/Generic/FinClassSetoid.lean
@@ -1,0 +1,32 @@
+import Mathlib.Data.Finset.Basic
+
+class FinClassSetoid (α : Type) extends Setoid α where
+  enumerateClass: α → Finset α
+  enumerateClass_mem_iff: ∀ x y, x ∈ enumerateClass y ↔ x ≈ y
+
+namespace FinClassSetoid
+
+lemma enumerateClass_self_mem [FinClassSetoid α] (x : α) : x ∈ enumerateClass x :=
+  (FinClassSetoid.enumerateClass_mem_iff x x).mpr (Setoid.refl x)
+
+theorem enumerateClass_eq [FinClassSetoid α] (x y : α) : enumerateClass x = enumerateClass y ↔ x ≈ y := by
+  apply Iff.intro
+  · intro h
+    have x_mem_enumerateClass_y : x ∈ enumerateClass y := by rw [←h]; exact enumerateClass_self_mem x
+    exact (enumerateClass_mem_iff x y).mp x_mem_enumerateClass_y
+  · intro h
+    ext a
+    apply Iff.intro
+    · intro h'
+      apply (enumerateClass_mem_iff _ _).mpr
+      apply (enumerateClass_mem_iff _ _).mp at h'
+      exact (Setoid.iseqv.trans h' h)
+    · intro h'
+      apply (enumerateClass_mem_iff _ _).mpr
+      apply (enumerateClass_mem_iff _ _).mp at h'
+      exact (Setoid.iseqv.trans h' (Setoid.iseqv.symm h))
+
+instance instEquivDecidable [FinClassSetoid α] [DecidableEq α] : DecidableRel ((· ≈ ·): α → α → Prop) := fun x y =>
+  decidable_of_decidable_of_iff (FinClassSetoid.enumerateClass_mem_iff x y)
+
+end FinClassSetoid
